WIP reducibility for internal histories

src/Reduction.v
@@ -13,58 +13,36 @@ Ltac dest_step_m :=
 Definition NonSilentHistory (hst: History) :=
   Forall (fun lbl => lbl <> emptyRLabel _) hst.
 
-Definition NotMsgsIn (lbl: MLabel) :=
+Definition Internal (lbl: MLabel) :=
   match lbl with
-  | RlblIns _ => False
-  | _ => True
+  | RlblInt _ _ _ => True
+  | _ => False
   end.
 
-Definition NonMsgsInHistory (hst: History) :=
-  Forall (fun tlbl => NotMsgsIn tlbl) hst.
-
-Definition NotMsgsOut (lbl: MLabel) :=
-  match lbl with
-  | RlblOuts _ => False
-  | _ => True
-  end.
-
-Definition NonMsgsOutHistory (hst: History) :=
-  Forall (fun tlbl => NotMsgsOut tlbl) hst.
+Definition InternalHistory (hst: History) :=
+  Forall (fun tlbl => Internal tlbl) hst.
 
 Lemma msg_ins_commutes:
   forall sys st1 eins lbl st2,
-    NotMsgsIn lbl ->
+    Internal lbl ->
     steps step_m sys st1 [RlblIns eins; lbl] st2 ->
     steps step_m sys st1 [lbl; RlblIns eins] st2.
 Proof.
   intros.
-  destruct lbl as [|hdl mins mouts|]; [elim H| |].
-  - dest_step_m.
+  destruct lbl as [|hdl mins mouts|]; [elim H| |elim H].
+  dest_step_m.
+  - econstructor.
     + econstructor.
-      * econstructor.
-        { econstructor. }
-        { econstructor; eauto. }
-      * econstructor.
+      * econstructor. 
+      * econstructor; eauto. 
     + econstructor.
-      * econstructor.
-        { econstructor. }
-        { econstructor; eauto. }
-      * econstructor; try reflexivity; try eassumption.
-        { clear -H9; induction mins; simpl; [constructor|].
-          inv H9; constructor; auto.
-          apply FirstMP_enqMsgs; auto.
-        }
-        { f_equal.
-          admit. (* requires a lemma about [MessagePool] *)
-        }
-  - dest_step_m.
-    econstructor.
+  - econstructor.
     + econstructor.
-      * econstructor.
-      * econstructor; eauto.
+      * econstructor. 
+      * econstructor; eauto. 
     + econstructor; try reflexivity; try eassumption.
-      * clear -H2; induction mouts; simpl; [constructor|].
-        inv H2; constructor; auto.
+      * clear -H9; induction mins; simpl; [constructor|].
+        inv H9; constructor; auto.
         apply FirstMP_enqMsgs; auto.
       * f_equal.
         admit. (* requires a lemma about [MessagePool] *)
@@ -73,7 +51,7 @@ Admitted.
 Lemma msg_in_reduced:
   forall sys st1 eins hst2 st2,
     steps step_m sys st1 (RlblIns eins :: hst2) st2 ->
-    NonMsgsInHistory hst2 ->
+    InternalHistory hst2 ->
     steps step_m sys st1 (hst2 ++ [RlblIns eins]) st2.
 Proof.
   induction hst2 as [|lbl ?]; simpl; intros; auto.
@@ -90,7 +68,7 @@ Qed.
 Lemma msg_in_reduced_app:
   forall sys st1 hst1 eins hst2 st2,
     steps step_m sys st1 (hst1 ++ RlblIns eins :: hst2) st2 ->
-    NonMsgsInHistory hst2 ->
+    InternalHistory hst2 ->
     steps step_m sys st1 (hst1 ++ hst2 ++ [RlblIns eins]) st2.
 Proof.
   intros.
@@ -102,55 +80,37 @@ Qed.
 
 Lemma msg_outs_commutes:
   forall sys st1 eouts lbl st2,
-    NotMsgsOut lbl ->
+    Internal lbl ->
     steps step_m sys st1 [lbl; RlblOuts eouts] st2 ->
     steps step_m sys st1 [RlblOuts eouts; lbl] st2.
 Proof.
   intros.
-  destruct lbl as [|hdl mins mouts|]; [| |elim H].
-  - dest_step_m.
-    econstructor.
-      * econstructor.
-        { econstructor. }
-        { econstructor; eauto. }
-      * econstructor; try reflexivity; try eassumption.
-        { clear -H2; induction eouts; simpl; [constructor|].
-          inv H2; constructor; auto.
-          apply FirstMP_enqMsgs; auto.
-        }
-        { f_equal.
-          admit. (* requires a lemma about [MessagePool] *)
-        }
-  - dest_step_m.
+  destruct lbl as [|hdl mins mouts|]; [elim H| |elim H].
+  dest_step_m.
+  - econstructor.
     + econstructor.
-      * econstructor.
-        { econstructor. }
-        { econstructor; eauto. }
-      * econstructor; eauto.
+      * econstructor. 
+      * econstructor; eauto. 
+    + econstructor; eauto.
+  - econstructor.
     + econstructor.
-      * econstructor.
-        { econstructor. }
-        { econstructor; try reflexivity; try eassumption.
-          admit. (* requires a lemma about [MessagePool] *)
-        }
+      * econstructor. 
       * econstructor; try reflexivity; try eassumption.
-        { admit. (* requires a lemma about [MessagePool] *)
-        }
-        { f_equal.
-          admit. (* requires a lemma about [MessagePool] *)
-        }
+        admit. (* requires a lemma about [MessagePool] *)
+    + econstructor; try reflexivity; try eassumption.
+      * admit. (* requires a lemma about [MessagePool] *)
+      * f_equal.
+        admit. (* requires a lemma about [MessagePool] *)
 Admitted.
 
 Lemma msg_outs_reduced:
   forall sys st1 eouts hst2 st2,
     steps step_m sys st1 (hst2 ++ [RlblOuts eouts]) st2 ->
-    NonMsgsOutHistory hst2 ->
+    InternalHistory hst2 ->
     steps step_m sys st1 (RlblOuts eouts :: hst2) st2.
 Proof.
   induction hst2 as [|lbl ?]; simpl; intros; auto.
-  inv H0.
-
-  inv H.
+  inv H0; inv H.
   specialize (IHhst2 _ H5 H4).
   assert (steps step_m sys st1 (lbl :: RlblOuts eouts :: hst2) st2)
     by (econstructor; eauto).
@@ -167,7 +127,7 @@ Qed.
 Lemma msg_outs_reduced_app:
   forall sys st1 hst1 eouts hst2 st2,
     steps step_m sys st1 (hst1 ++ hst2 ++ [RlblOuts eouts]) st2 ->
-    NonMsgsOutHistory hst2 ->
+    InternalHistory hst2 ->
     steps step_m sys st1 (hst1 ++ RlblOuts eouts :: hst2) st2.
 Proof.
   intros.
