src/PredMsg.v
@@ -185,7 +185,7 @@ Definition pToTHistory (phst: PHistory TMsg): THistory :=
 
 Definition PTStateR (tst: TState) (pst: PState TMsg) :=
   tst_oss tst = pst_oss pst /\
-  tst_orqs tst = M.map (map (@pmsg_omsg _)) (pst_orqs pst) /\
+  tst_orqs tst = M.map (imap (@pmsg_omsg _)) (pst_orqs pst) /\
   tst_msgs tst = M.map (map (@pmsg_omsg _)) (pst_msgs pst).
 
 Section RuleAdder.
